More debugging attempts for heaplet API

vale/code/arch/x64/Vale.X64.State.fsti
@@ -87,8 +87,7 @@ let update_reg_xmm (r:reg_xmm) (v:quad32) (s:vale_state) : vale_state =
 let update_mem (ptr:int) (v:nat64) (s:vale_state) : GTot vale_state = {s with vs_heap = store_mem64 ptr v s.vs_heap}
 
 [@va_qattr]
-let update_heap (hp: nat) (h: vale_heap) (s:vale_state) : vale_state =
-  {s with vs_hpls = Map.upd s.vs_hpls hp h}
+let update_heap (hp: nat) (h: vale_heap) (s:vale_state) : vale_state = {s with vs_hpls = Map.upd s.vs_hpls hp h }
   
 [@va_qattr]
 let update_stack64 (ptr:int) (v:nat64) (s:vale_state) : GTot vale_state = {s with vs_stack = store_stack64 ptr v s.vs_stack}
