vale/code/arch/x64/Vale.X64.Decls.fsti
@@ -257,6 +257,7 @@ val taint_at (memTaint:M.memtaint) (addr:int) : taint
 [@va_qattr] unfold let va_is_dst_reg_opr64 (o:va_operand) (s:va_state) = OReg? o /\ not (rRsp = (OReg?.r o))
 [@va_qattr] unfold let va_is_src_xmm (x:reg_xmm) (s:va_state) = True
 [@va_qattr] unfold let va_is_src_heap (hp:nat) (s:va_state) = True
+[@va_qattr] unfold let va_is_dst_heap (hp:nat) (s:va_state) = True
 [@va_qattr] unfold let va_is_dst_xmm (x:reg_xmm) (s:va_state) = True
 [@va_qattr] unfold let va_is_src_opr128 (o:va_operand128) (s:va_state) = valid_operand128 o s
 [@va_qattr] unfold let va_is_dst_opr128 (o:va_operand128) (s:va_state) = valid_operand128 o s
@@ -278,7 +279,7 @@ val taint_at (memTaint:M.memtaint) (addr:int) : taint
 [@va_qattr] let va_upd_reg64 (r:reg_64) (v:nat64) (s:vale_state) : vale_state = update_reg_64 r v s
 [@va_qattr] let va_upd_xmm (x:reg_xmm) (v:quad32) (s:vale_state) : vale_state = update_reg_xmm x v s
 [@va_qattr] let va_upd_mem (mem:vale_heap) (s:vale_state) : vale_state = { s with vs_heap = mem }
-[@va_qattr] let va_upd_heap (hp:nat) (h:vale_heap) (s:vale_state) : vale_state = { s with vs_hpls = Map.upd s.vs_hpls hp h }
+[@va_qattr] let va_upd_heap (hp:nat) (h:vale_heap) (s:vale_state) : vale_state = update_heap hp h s
 [@va_qattr] let va_upd_stack (stack:S.vale_stack) (s:vale_state) : vale_state = { s with vs_stack = stack }
 [@va_qattr] let va_upd_memTaint (memTaint:M.memtaint) (s:vale_state) : vale_state = { s with vs_memTaint = memTaint }
 [@va_qattr] let va_upd_stackTaint (stackTaint:M.memtaint) (s:vale_state) : vale_state = { s with vs_stackTaint = stackTaint }
